Rework syntax

src/FJ/Syntax.v
@@ -52,19 +52,28 @@ Inductive Assignment :=
 Inductive Constructor :=
   | KDecl : id -> [FormalArg] -> [Argument] -> [Assignment] -> Constructor.
 
+Inductive ConstructorRefine :=
+  | KRefine : id -> [FormalArg] -> [Argument] -> [Assignment] -> ConstructorRefine.
 
-(* Arguments cannot have duplicate names *)
+
 Inductive MethodDecl :=
-  | MDecl : ClassName -> id -> forall (fargs: [FormalArg]), NoDup (this :: refs fargs) -> Exp -> MethodDecl.
+  (* MDecl is the return of the method, its name and nonduplicate list of formal args *)
+  | MDecl : ClassName -> id -> forall (fargs: [FormalArg]), NoDup (this :: refs fargs) -> Exp -> MethodDecl
+  (* MRefine is the same *)
+  | MRefine : ClassName -> id -> forall (fargs: [FormalArg]), NoDup (this :: refs fargs) -> Exp -> MethodDecl
+.
 
 
 Instance MDeclRef : Referable MethodDecl :={
   ref mdecl := 
     match mdecl with 
-   | MDecl _ id _ _ _ => id end
+   | MDecl _ id _ _ _ => id
+   | MRefine _ id _ _ _ => id end
 }.
 
-Inductive ClassDecl:=
+Inductive ClassDecl :=
+  (* CDecl is the name of the class, the superclass, non duplicate fields,
+  constructor and non duplicate methods *)
   | CDecl: id -> ClassName -> 
     forall (fDecls:[FieldDecl]), NoDup (refs fDecls) -> Constructor -> 
     forall (mDecls:[MethodDecl]), NoDup (refs mDecls) -> ClassDecl.
@@ -75,8 +84,38 @@ Instance CDeclRef : Referable ClassDecl :={
    | CDecl id _ _ _ _ _ _ => id end
 }.
 
-Inductive Program :=
-  | CProgram : forall (cDecls: [ClassDecl]), NoDup (refs cDecls) -> Exp -> Program.
+(* The Name of a feature also encodes its order, taken from the "composition engine" *)
+Definition FeatureName := nat.
 
-(* We assume a fixed ClassTable *)
-Parameter CT: [ClassDecl].
+Inductive RefinementName :=
+  | RName : id -> FeatureName -> RefinementName.
+
+Notation "C @ Feat" := (RName C Feat) (at level 30).
+
+Inductive ClassRefinement :=
+  (* CRefine is the name of the class
+  , non duplicate fields,
+  constructor and non duplicate methods *)
+  | CRefine: id -> FeatureName ->
+    forall (fDecls:[FieldDecl]), NoDup (refs fDecls) -> ConstructorRefine -> 
+    forall (mDecls:[MethodDecl]), NoDup (refs mDecls) -> ClassRefinement.
+
+Instance CRefinementRef : Referable ClassRefinement :={
+  ref cdecl := 
+    match cdecl with 
+   | (CRefine id _ _ _ _ _ _) => id end
+}.
+
+Inductive Class :=
+  | CD : ClassDecl -> Class
+  | CR : ClassRefinement -> Class.
+
+Instance CRef : Referable Class :={
+  ref cdecl := 
+    match cdecl with 
+   | CD CDe => ref CDe
+   | CR CRefinement => ref CRefinement end
+}.
+
+Inductive Program :=
+  | CProgram : forall (cDecls: [Class]), NoDup (refs cDecls) -> Exp -> Program.
